Move to iris-3.5

theories/Model.v
@@ -54,8 +54,7 @@ From iris.base_logic Require Export invariants.
 From iris.bi Require interface big_op.
 From iris.algebra Require dfrac.
 From iris.program_logic Require Import weakestpre adequacy.
-From iris.proofmode Require Import tactics.
-From iris_string_ident Require Import ltac2_string_ident.
+From iris.proofmode Require Import string_ident tactics.
 From stdpp Require namespaces fin_maps.
 
 Set Implicit Arguments.
@@ -106,21 +105,22 @@ Module MinCapsModel.
 
     Definition MemVal : Set := Z + Capability.
 
-    Class mcMemG Σ := McMemG {
+    Class mcMemGS Σ := McMemGS {
                           (* ghost variable for tracking state of registers *)
-                          mc_ghG :> gh.gen_heapG Z MemVal Σ;
+                          mc_ghG :> gh.gen_heapGS Z MemVal Σ;
                           mc_invNs : namespace
                         }.
 
-    Definition memPreG : gFunctors -> Set := fun Σ => gh.gen_heapPreG Z MemVal Σ.
-    Definition memG : gFunctors -> Set := mcMemG.
+    Definition memGpreS : gFunctors -> Set := fun Σ => gh.gen_heapGpreS Z MemVal Σ.
+    Definition memGS : gFunctors -> Set := mcMemGS.
     Definition memΣ : gFunctors := gh.gen_heapΣ Z MemVal.
 
-    Definition memΣ_PreG : forall {Σ}, subG memΣ Σ -> memPreG Σ := fun {Σ} => gh.subG_gen_heapPreG (Σ := Σ) (L := Z) (V := MemVal).
+    Definition memΣ_GpreS : forall {Σ}, subG memΣ Σ -> memGpreS Σ :=
+      fun {Σ} => gh.subG_gen_heapGpreS (Σ := Σ) (L := Z) (V := MemVal).
 
-    Definition mem_inv : forall {Σ}, memG Σ -> Memory -> iProp Σ :=
+    Definition mem_inv : forall {Σ}, memGS Σ -> Memory -> iProp Σ :=
       fun {Σ} hG μ =>
-        (∃ memmap, gen_heap_interp (hG := mc_ghG (mcMemG := hG)) memmap ∗
+        (∃ memmap, gen_heap_interp (hG := mc_ghG (mcMemGS := hG)) memmap ∗
                                 ⌜ map_Forall (fun a v => μ a = v) memmap ⌝
         )%I.
 
@@ -141,23 +141,23 @@ Module MinCapsModel.
       by destruct el as (a' & <- & _).
     Qed.
 
-    Definition mem_res : forall {Σ}, memG Σ -> Memory -> iProp Σ :=
+    Definition mem_res : forall {Σ}, memGS Σ -> Memory -> iProp Σ :=
       fun {Σ} hG μ =>
-        ([∗ map] l↦v ∈ initMemMap μ, mapsto (hG := mc_ghG (mcMemG := hG)) l (DfracOwn 1) v) %I.
+        ([∗ map] l↦v ∈ initMemMap μ, mapsto (hG := mc_ghG (mcMemGS := hG)) l (DfracOwn 1) v) %I.
 
-    Lemma mem_inv_init : forall Σ (μ : Memory), memPreG Σ ->
-        ⊢ |==> ∃ memG : memG Σ, (mem_inv memG μ ∗ mem_res memG μ)%I.
+    Lemma mem_inv_init : forall Σ (μ : Memory), memGpreS Σ ->
+      ⊢ |==> ∃ mG : memGS Σ, (mem_inv mG μ ∗ mem_res mG μ)%I.
     Proof.
       iIntros (Σ μ gHP).
 
-      iMod (gen_heap_init (gen_heapPreG0 := gHP) (L := Addr) (V := MemVal) empty) as (gH) "[inv _]".
+      iMod (gen_heap_init (gen_heapGpreS0 := gHP) (L := Addr) (V := MemVal) empty) as (gH) "[inv _]".
       pose (memmap := initMemMap μ).
       iMod (gen_heap_alloc_big empty memmap (map_disjoint_empty_r memmap) with "inv") as "(inv & res & _)".
       iModIntro.
 
       rewrite (right_id empty union memmap).
 
-      iExists (McMemG gH (nroot .@ "addr_inv")).
+      iExists (McMemGS gH (nroot .@ "addr_inv")).
       iFrame.
       iExists memmap.
       iFrame.
@@ -165,7 +165,7 @@ Module MinCapsModel.
       apply initMemMap_works.
     Qed.
 
-    Definition MinCaps_ptsreg `{sailRegG Σ} (reg : RegName) (v : Z + Capability) : iProp Σ :=
+    Definition MinCaps_ptsreg `{sailRegGS Σ} (reg : RegName) (v : Z + Capability) : iProp Σ :=
       match reg with
       | R0 => reg_pointsTo reg0 v
       | R1 => reg_pointsTo reg1 v
@@ -173,7 +173,7 @@ Module MinCapsModel.
       | R3 => reg_pointsTo reg3 v
       end.
 
-    Lemma MinCaps_ptsreg_regtag_to_reg `{sailRegG Σ} (reg : RegName) (v : Z + Capability) :
+    Lemma MinCaps_ptsreg_regtag_to_reg `{sailRegGS Σ} (reg : RegName) (v : Z + Capability) :
       MinCaps_ptsreg reg v = reg_pointsTo (regtag_to_reg reg) v.
     Proof.
       by destruct reg.
@@ -218,37 +218,37 @@ Module MinCapsModel.
 
     Ltac solve_proper ::= (repeat intros ?; simpl; auto_equiv).
 
-    Program Definition MinCaps_ref_inv `{sailRegG Σ} `{invG Σ} {mG : memG Σ} (a : Addr) : D -n> iPropO Σ :=
-      λne P, (∃ w, mapsto (hG := mc_ghG (mcMemG := mG)) a (DfracOwn 1) w ∗ P w)%I.
+    Program Definition MinCaps_ref_inv `{sailRegGS Σ} `{invGS Σ} {mG : memGS Σ} (a : Addr) : D -n> iPropO Σ :=
+      λne P, (∃ w, mapsto (hG := mc_ghG (mcMemGS := mG)) a (DfracOwn 1) w ∗ P w)%I.
     Solve All Obligations with solve_proper.
 
-    Program Definition MinCaps_csafe `{sailRegG Σ} `{invG Σ} {mG : memG Σ} (safe : D) : D :=
+    Program Definition MinCaps_csafe `{sailRegGS Σ} `{invGS Σ} {mG : memGS Σ} (safe : D) : D :=
       λne w,
         (match w with
         | inr (MkCap O b e a) => True%I
         | inr (MkCap R b e a) =>
           (⌜ (b <= e)%Z ⌝ →
             ⌜ b ∈ liveAddrs /\ e ∈ liveAddrs ⌝ ∗
-                                [∗ list] a ∈ (region_addrs b e), inv (mc_invNs (mcMemG := mG) .@ a) (MinCaps_ref_inv (mG := mG) a safe))
+                                [∗ list] a ∈ (region_addrs b e), inv (mc_invNs (mcMemGS := mG) .@ a) (MinCaps_ref_inv (mG := mG) a safe))
           ∨
           ⌜ (e < b)%Z ⌝
         | inr (MkCap RW b e a) =>
           (⌜ (b <= e)%Z ⌝ →
             ⌜ b ∈ liveAddrs /\ e ∈ liveAddrs ⌝ ∗
-                                [∗ list] a ∈ (region_addrs b e), inv (mc_invNs (mcMemG := mG) .@ a) (MinCaps_ref_inv (mG := mG) a safe))
+                                [∗ list] a ∈ (region_addrs b e), inv (mc_invNs (mcMemGS := mG) .@ a) (MinCaps_ref_inv (mG := mG) a safe))
           ∨
           ⌜ (e < b)%Z ⌝
         | inl _ => False
         end)%I.
 
-    Program Definition MinCaps_safe1 `{sailRegG Σ} `{invG Σ} {mG : memG Σ} (safe : D) : D :=
+    Program Definition MinCaps_safe1 `{sailRegGS Σ} `{invGS Σ} {mG : memGS Σ} (safe : D) : D :=
       λne w,
         (match w with
         | inl z => True
         | inr c => MinCaps_csafe (mG := mG) safe w
         end)%I.
 
-    Global Instance MinCaps_csafe_contractive `{sailRegG Σ} `{invG Σ} {mG : memG Σ} :
+    Global Instance MinCaps_csafe_contractive `{sailRegGS Σ} `{invGS Σ} {mG : memGS Σ} :
       Contractive (MinCaps_csafe (mG := mG)).
     Proof.
       intros n x y Hdist w.
@@ -258,7 +258,7 @@ Module MinCapsModel.
       destruct cap_permission; first auto; solve_proper_prepare; solve_contractive.
     Qed.
 
-    Global Instance MinCaps_safe1_contractive `{sailRegG Σ} `{invG Σ} {mG : memG Σ} :
+    Global Instance MinCaps_safe1_contractive `{sailRegGS Σ} `{invGS Σ} {mG : memGS Σ} :
       Contractive (MinCaps_safe1 (mG := mG)).
     Proof.
       intros n x y Hdist w.
@@ -267,11 +267,11 @@ Module MinCapsModel.
       by apply MinCaps_csafe_contractive.
     Qed.
 
-    Lemma fixpoint_MinCaps_safe1_eq `{sailRegG Σ} `{invG Σ} {mG : memG Σ} (w : leibnizO MemVal) :
+    Lemma fixpoint_MinCaps_safe1_eq `{sailRegGS Σ} `{invGS Σ} {mG : memGS Σ} (w : leibnizO MemVal) :
       fixpoint (MinCaps_safe1 (mG := mG)) w ≡ MinCaps_safe1 (mG := mG) (fixpoint (MinCaps_safe1 (mG := mG))) w.
     Proof. exact: (fixpoint_unfold (MinCaps_safe1 (mG := mG)) w). Qed.
 
-    Definition MinCaps_safe `{sailRegG Σ} `{invG Σ} {mG : memG Σ} : D :=
+    Definition MinCaps_safe `{sailRegGS Σ} `{invGS Σ} {mG : memGS Σ} : D :=
       λne w, (fixpoint (MinCaps_safe1 (mG := mG))) w.
 
     Lemma le_liveAddrs (a b e : Addr) :
@@ -288,13 +288,14 @@ Module MinCapsModel.
       split; lia.
     Qed.
 
-    Lemma region_addrs_submseteq `{sailRegG Σ} `{invG Σ} {mG : memG Σ} (b' e' b e : Addr) :
+    Lemma region_addrs_submseteq `{sailRegGS Σ} `{invGS Σ} {mG : memGS Σ} (b' e' b e : Addr) :
       ⊢ ⌜ (b <= b')%Z /\ (e' <= e)%Z ⌝ -∗
-                               ([∗ list] a ∈ (region_addrs b e), inv (mc_invNs (mcMemG := mG) .@ a) (∃ w, mapsto (hG := mc_ghG (mcMemG := mG)) a (DfracOwn 1) w ∗ fixpoint (MinCaps_safe1 (mG := mG)) w))%I -∗
-                               ([∗ list] a ∈ (region_addrs b' e'), inv (mc_invNs (mcMemG := mG) .@ a) (∃ w, mapsto (hG := mc_ghG (mcMemG := mG)) a (DfracOwn 1) w ∗ fixpoint (MinCaps_safe1 (mG := mG)) w))%I.
+                               ([∗ list] a ∈ (region_addrs b e), inv (mc_invNs (mcMemGS := mG) .@ a) (∃ w, mapsto (hG := mc_ghG (mcMemGS := mG)) a (DfracOwn 1) w ∗ fixpoint (MinCaps_safe1 (mG := mG)) w))%I -∗
+                               ([∗ list] a ∈ (region_addrs b' e'), inv (mc_invNs (mcMemGS := mG) .@ a) (∃ w, mapsto (hG := mc_ghG (mcMemGS := mG)) a (DfracOwn 1) w ∗ fixpoint (MinCaps_safe1 (mG := mG)) w))%I.
     Proof.
       iIntros "[% %] Hregion".
-      iApply (big_sepL_submseteq _ _ (region_addrs b e)).
+      iApply (big_sepL_submseteq _ (region_addrs b' e') (region_addrs b e)).
+      Unshelve. all: eauto with typeclass_instances.
       unfold region_addrs.
       induction liveAddrs.
       - cbn; trivial.
@@ -305,10 +306,9 @@ Module MinCapsModel.
         + apply submseteq_skip; trivial.
         + destruct a0 as [Hb' He']; lia.
         + apply submseteq_cons; trivial.
-      - iAssumption.
     Qed.
 
-    Lemma safe_sub_range `{sailRegG Σ} `{invG Σ} {mG : memG Σ} (b' e' b e : Addr) :
+    Lemma safe_sub_range `{sailRegGS Σ} `{invGS Σ} {mG : memGS Σ} (b' e' b e : Addr) :
       forall p a,
       ⊢ ⌜ (b <= b')%Z /\ (e' <= e)%Z ⌝ -∗
                                MinCaps_safe (mG := mG)
@@ -358,11 +358,11 @@ Module MinCapsModel.
         + iApply (region_addrs_submseteq $! (conj H1 H2) with "H").
     Qed.
 
-    Lemma specialize_range `{sailRegG Σ} `{invG Σ} {mG : memG Σ} (b e addr : Addr) :
+    Lemma specialize_range `{sailRegGS Σ} `{invGS Σ} {mG : memGS Σ} (b e addr : Addr) :
       ⊢ ⌜ (b <= addr)%Z /\ (addr <= e)%Z ⌝ -∗
         (⌜ b ∈ liveAddrs /\ e ∈ liveAddrs ⌝ ∗
-          [∗ list] a ∈ (region_addrs b e), inv (mc_invNs (mcMemG := mG) .@ a) (∃ w, mapsto (hG := mc_ghG (mcMemG := mG)) a (DfracOwn 1) w ∗ fixpoint (MinCaps_safe1 (mG := mG)) w))%I -∗
-        (inv (mc_invNs (mcMemG := mG) .@ addr) (∃ w, mapsto (hG := mc_ghG (mcMemG := mG)) addr (DfracOwn 1) w ∗ fixpoint (MinCaps_safe1 (mG := mG)) w))%I.
+          [∗ list] a ∈ (region_addrs b e), inv (mc_invNs (mcMemGS := mG) .@ a) (∃ w, mapsto (hG := mc_ghG (mcMemGS := mG)) a (DfracOwn 1) w ∗ fixpoint (MinCaps_safe1 (mG := mG)) w))%I -∗
+        (inv (mc_invNs (mcMemGS := mG) .@ addr) (∃ w, mapsto (hG := mc_ghG (mcMemGS := mG)) addr (DfracOwn 1) w ∗ fixpoint (MinCaps_safe1 (mG := mG)) w))%I.
     Proof.
       iIntros "[% %] [[% %] Hrange]".
       iApply (big_sepL_elem_of with "Hrange").
@@ -372,25 +372,25 @@ Module MinCapsModel.
 
     Definition GPRs : list RegName := finite.enum RegName.
 
-    Definition interp_gprs `{sailRegG Σ} `{invG Σ} `{mG : memG Σ} : iProp Σ :=
+    Definition interp_gprs `{sailRegGS Σ} `{invGS Σ} `{mG : memGS Σ} : iProp Σ :=
       [∗ list] r ∈ GPRs, (∃ w, MinCaps_ptsreg r w ∗ MinCaps_safe (mG := mG) w)%I.
 
     Import env.notations.
 
-    Definition luser_inst `{sailRegG Σ} `{invG Σ} (mG : memG Σ) (p : Predicate) (ts : Env Val (𝑯_Ty p)) : iProp Σ :=
+    Definition luser_inst `{sailRegGS Σ} `{invGS Σ} (mG : memGS Σ) (p : Predicate) (ts : Env Val (𝑯_Ty p)) : iProp Σ :=
       (match p return Env Val (𝑯_Ty p) -> iProp Σ with
       | ptsreg => fun ts => MinCaps_ptsreg (env.head (env.tail ts)) (env.head ts)
-      | ptsto => fun ts => mapsto (hG := mc_ghG (mcMemG := mG)) (env.head (env.tail ts)) (DfracOwn 1) (env.head ts)
+      | ptsto => fun ts => mapsto (hG := mc_ghG (mcMemGS := mG)) (env.head (env.tail ts)) (DfracOwn 1) (env.head ts)
       | safe => fun ts => MinCaps_safe (mG := mG) (env.head ts)
       | dummy => fun ts => True%I
       | gprs => fun ts => interp_gprs (mG := mG)
       end) ts.
 
-    Global Instance MinCaps_safe_Persistent `{sailRegG Σ} `{invG Σ} {mG : memG Σ} (w : leibnizO MemVal) : Persistent (MinCaps_safe (mG := mG) w).
+    Global Instance MinCaps_safe_Persistent `{sailRegGS Σ} `{invGS Σ} {mG : memGS Σ} (w : leibnizO MemVal) : Persistent (MinCaps_safe (mG := mG) w).
     Proof. destruct w; simpl; rewrite fixpoint_MinCaps_safe1_eq; simpl; first apply _.
            destruct c; destruct cap_permission; apply _. Qed.
 
-    Definition lduplicate_inst `{sailRegG Σ} `{invG Σ} (mG : memG Σ) :
+    Definition lduplicate_inst `{sailRegGS Σ} `{invGS Σ} (mG : memGS Σ) :
       forall (p : Predicate) (ts : Env Val (𝑯_Ty p)),
         is_duplicable p = true ->
         (luser_inst mG p ts) ⊢ (luser_inst mG p ts ∗ luser_inst mG p ts).
@@ -407,7 +407,7 @@ Module MinCapsModel.
   Module Import MinCapsIrisInstance := IrisInstance MinCapsIrisHeapKit.
 
   Section Lemmas.
-    Context `{sg : sailG Σ}.
+    Context `{sg : sailGS Σ}.
 
     Lemma gen_dummy_sound :
       ValidLemma MinCapsSpecification.lemma_gen_dummy.
@@ -504,7 +504,7 @@ Module MinCapsModel.
 
   End Lemmas.
 
-  Lemma dI_sound `{sg : sailG Σ} `{invG} {Γ es δ} :
+  Lemma dI_sound `{sg : sailGS Σ} `{invGS} {Γ es δ} :
     forall code : Val ty_int,
     evals es δ = env.snoc env.nil (MkB _ ty_int) code
     → ⊢ semTriple δ (⌜is_true true⌝ ∧ emp) (stm_foreign dI es)
@@ -523,21 +523,21 @@ Module MinCapsModel.
 
   Import iris.base_logic.lib.gen_heap.
 
-  Lemma rM_sound `{sg : sailG Σ} `{invG} {Γ es δ} :
+  Lemma rM_sound `{sg : sailGS Σ} `{invGS} {Γ es δ} :
     forall a (p : Val ty_perm) (b e : Val ty_addr),
       evals es δ = env.snoc env.nil (MkB _ ty_addr) a ->
     ⊢ semTriple δ
-        (MinCapsIrisHeapKit.MinCaps_safe (mG := sailG_memG)
+        (MinCapsIrisHeapKit.MinCaps_safe (mG := sailGS_memGS)
            (inr {| cap_permission := p; cap_begin := b; cap_end := e; cap_cursor := a |})
          ∗ (⌜Subperm R p⌝ ∧ emp) ∗ ⌜(b <=? a)%Z && (a <=? e)%Z = true⌝ ∧ emp)
         (stm_foreign rM es)%env
         (λ (v : Z + Capability) (δ' : CStore Γ),
-           (MinCapsIrisHeapKit.MinCaps_safe (mG := sailG_memG) v) ∗ ⌜δ' = δ⌝).
+           (MinCapsIrisHeapKit.MinCaps_safe (mG := sailGS_memGS) v) ∗ ⌜δ' = δ⌝).
   Proof.
     intros a p b e Heq.
     iIntros "[#Hsafe [[%Hsubp _] [%Hbounds _]]]".
     apply andb_prop in Hbounds as [Hb%Zle_is_le_bool He%Zle_is_le_bool].
-    rewrite wp_unfold.
+    rewrite wp_unfold. cbn.
     destruct p; try discriminate.
     (* TODO: clean this up! *)
     - iAssert (inv (MinCapsIrisHeapKit.mc_invNs.@a) (∃ w, gen_heap.mapsto a (dfrac.DfracOwn 1) w ∗ MinCapsIrisHeapKit.MinCaps_safe w))%I as "Hown".
@@ -553,19 +553,18 @@ Module MinCapsModel.
         )%I with "[Htmp Hsafe]" as "Hsafe'".
         { iApply ("Hsafe" with "Htmp"). }
         iApply (MinCapsIrisHeapKit.specialize_range $! (conj Hb He) with "Hsafe'"). }
-      iIntros (σ' ks1 ks n) "[Hregs Hmem]".
+      iIntros (σ' ns ks1 ks nt) "[Hregs Hmem]".
       iDestruct "Hmem" as (memmap) "[Hmem' %]".
       iInv "Hown" as "Hinv" "Hclose".
       iMod (fupd_mask_subseteq empty) as "Hclose2"; first set_solver.
       iModIntro.
       iSplitR; first by intuition.
       iIntros (e2 σ'' efs) "%".
-      cbn in H1.
       dependent elimination H1.
       dependent elimination s.
       cbn in f1.
       dependent elimination f1.
-      do 2 iModIntro.
+      do 3 iModIntro.
       iDestruct "Hinv" as (v) "Hav".
       iDestruct "Hav" as "[Hav #Hrec]".
       iAssert (⌜ memmap !! a = Some v ⌝)%I with "[Hav Hmem']" as "%".
@@ -601,19 +600,18 @@ Module MinCapsModel.
         )%I with "[Htmp Hsafe]" as "Hsafe'".
         { iApply ("Hsafe" with "Htmp"). }
         iApply (MinCapsIrisHeapKit.specialize_range $! (conj Hb He) with "Hsafe'"). }
-      iIntros (σ' ks1 ks n) "[Hregs Hmem]".
+      iIntros (σ' ns ks1 ks nt) "[Hregs Hmem]".
       iDestruct "Hmem" as (memmap) "[Hmem' %]".
       iInv "Hown" as "Hinv" "Hclose".
       iMod (fupd_mask_subseteq empty) as "Hclose2"; first set_solver.
       iModIntro.
       iSplitR; first by intuition.
       iIntros (e2 σ'' efs) "%".
-      cbn in H1.
       dependent elimination H1.
       dependent elimination s.
       cbn in f1.
       dependent elimination f1.
-      do 2 iModIntro.
+      do 3 iModIntro.
       iDestruct "Hinv" as (v) "Hav".
       iDestruct "Hav" as "[Hav #Hrec]".
       iAssert (⌜ memmap !! a = Some v ⌝)%I with "[Hav Hmem']" as "%".
@@ -638,13 +636,13 @@ Module MinCapsModel.
       iAssumption.
   Qed.
 
-  Lemma wM_sound `{sg : sailG Σ} `{invG} {Γ es δ} :
+  Lemma wM_sound `{sg : sailGS Σ} `{invGS} {Γ es δ} :
     forall a w (p : Val ty_perm) (b e : Val ty_addr),
       evals es δ = env.snoc (env.snoc env.nil (MkB _ ty_addr) a)
                             (MkB _ ty_memval) w
     → ⊢ semTriple δ
-        (MinCapsIrisHeapKit.MinCaps_safe (mG := sailG_memG) w
-         ∗ MinCapsIrisHeapKit.MinCaps_safe (mG := sailG_memG)
+        (MinCapsIrisHeapKit.MinCaps_safe (mG := sailGS_memGS) w
+         ∗ MinCapsIrisHeapKit.MinCaps_safe (mG := sailGS_memGS)
                                           (inr {|
                                                cap_permission := p;
                                                cap_begin := b;
@@ -659,9 +657,9 @@ Module MinCapsModel.
       intros a w p b e Heq.
       iIntros "[#Hwsafe [#Hsafe [[%Hsubp _] [%Hbounds _]]]]".
       apply andb_prop in Hbounds as [Hb%Zle_is_le_bool He%Zle_is_le_bool].
-      rewrite wp_unfold.
+      rewrite wp_unfold. cbn.
       destruct p; try discriminate. clear Hsubp.
-      iIntros (σ' ks1 ks n) "[Hregs Hmem]".
+      iIntros (σ' ns ks1 ks nt) "[Hregs Hmem]".
       iDestruct "Hmem" as (memmap) "[Hmem' %]".
       iAssert (inv (MinCapsIrisHeapKit.mc_invNs.@a) (∃ w, gen_heap.mapsto a (dfrac.DfracOwn 1) w ∗ fixpoint (MinCapsIrisHeapKit.MinCaps_safe1) w))%I as "Hown".
       { do 2 rewrite MinCapsIrisHeapKit.fixpoint_MinCaps_safe1_eq; simpl.
@@ -681,13 +679,12 @@ Module MinCapsModel.
       iModIntro.
       iSplitR; first by intuition.
       iIntros (e2 σ'' efs) "%".
-      cbn in H1.
       dependent elimination H1.
       dependent elimination s.
       rewrite Heq in f1.
       cbn in f1.
       dependent elimination f1.
-      do 2 iModIntro.
+      do 3 iModIntro.
       iDestruct "Hinv" as (v) "Hav".
       iDestruct "Hav" as "[Hav Hrec]".
       iMod (gen_heap.gen_heap_update _ _ _ w with "Hmem' Hav") as "[Hmem' Hav]".
@@ -719,7 +716,7 @@ Module MinCapsModel.
           repeat (iSplitL; trivial).
     Qed.
 
-  Lemma foreignSem `{sg : sailG Σ} : ForeignSem (Σ := Σ).
+  Lemma foreignSem `{sg : sailGS Σ} : ForeignSem (Σ := Σ).
   Proof.
     intros Γ τ Δ f es δ.
     destruct f; cbn - [MinCapsIrisHeapKit.MinCaps_safe MinCapsIrisHeapKit.MinCaps_csafe];
@@ -727,7 +724,7 @@ Module MinCapsModel.
         eauto using dI_sound, rM_sound, wM_sound.
   Qed.
 
-  Lemma lemSem `{sg : sailG Σ} : LemmaSem (Σ := Σ).
+  Lemma lemSem `{sg : sailGS Σ} : LemmaSem (Σ := Σ).
   Proof.
     intros Δ []; eauto using
       open_ptsreg_sound, close_ptsreg_sound,
